# Esercizi sulle equazioni di secondo grado

| Equazione | Soluzione |
|----------|-----------|
| \( x^2 - 4 = 0 \) | \( \{-2,\ 2\} \) |
| \( x^2 = 0 \) | \( \{0\} \) |
| \( 2x^2 - 8 = 0 \) | \( \{-2,\ 2\} \) |
| \( -x^2 - 4 = 0 \) | impossibile |
| \( x^2 + 2x = 0 \) | \( \{-2,\ 0\} \) |
| \( x^2 - x = 0 \) | \( \{0,\ 1\} \) |
| \( -2x^2 + 4x = 0 \) | \( \{0,\ 2\} \) |
| \( 3x^2 + 6x = 0 \) | \( \{-2,\ 0\} \) |
| \( x^2 + 4x + 4 = 0 \) | \( \{-2\} \) |
| \( x^2 + x - 2 = 0 \) | \( \{-1,\ 2\} \) |
| \( x^2 - 3x + 2 = 0 \) | \( \{1,\ 2\} \) |
| \( -x^2 + 2x - 1 = 0 \) | \( \{1\} \) |
| \( 2x^2 + 6x + 4 = 0 \) | \( \{-2,\ -1\} \) |
| \( 2x^2 - 2 = 0 \) | \( \{-1,\ 1\} \) |
| \( -2x^2 - 4x - 2 = 0 \) | \( \{-1\} \) |
| \( 2x^2 - 6x + 4 = 0 \) | \( \{1,\ 2\} \) |
| \( -2x^2 + 8x - 8 = 0 \) | \( \{2\} \) |
| \( 3x^2 + 2x - 1 = 0 \) | \( \{-1,\ \tfrac{1}{3}\} \) |
