# Equazioni di 1Â° grado

| Equazione | Soluzione |
|----------|-----------|
| \(3x + 1 = 4\) | \(x = 1\) |
| \(5 = 5x + 3(3x + 1)\) | \(x = \tfrac{1}{7}\) |
| \(8(2x + 1) + 4 = 6\) | \(x = -\tfrac{3}{8}\) |
| \(6x + 8 = 3x + 6\) | \(x = -\tfrac{2}{3}\) |
| \(x + 10(x + 1) + 2 = 2x + 5\) | \(x = -\tfrac{7}{9}\) |
| \(x + 3 = 2(2x + 3)\) | \(x = -1\) |
| \(5x + 5(2x + 5) + 12 = 4x + 5\) | \(x = -\tfrac{32}{11}\) |
| \(6x + 5 = x + 8(2x + 1)\) | \(x = -\tfrac{3}{11}\) |
| \(2(2x + 1) + 2(5x + 4) + 2 = x + 2\) | \(x = -\tfrac{10}{13}\) |
| \(7 = 12x + 4\) | \(x = \tfrac{1}{4}\) |
| \(12x + 1 = 5x + 2\) | \(x = \tfrac{1}{7}\) |
| \(3(x + 5) + 4(2x + 1) + 4 = 3x\) | \(x = -\tfrac{23}{8}\) |
| \(5x + 6(x + 1) + 3 = 4x + 7\) | \(x = -\tfrac{2}{7}\) |
| \(x + 3(4x + 5) = 5x + 3\) | \(x = -\tfrac{3}{2}\) |
| \(x + 5 = 5\) | \(x = 0\) |
| \(7x + 1 = 0\) | \(x = -\tfrac{1}{7}\) |
| \(5x + 3(x + 5) + 3 = 0\) | \(x = -\tfrac{9}{4}\) |
| \(2x + 3(5x + 1) = 12\) | \(x = \tfrac{9}{17}\) |
| \( \frac{2(2 - 2x)}{3} - 1 = -x - 3 \) | \( x = 10 \) |
| \( \frac{5x}{2} = \frac{-2x - 1}{2} + 2 \) | \( x = \tfrac{3}{7} \) |
| \( \frac{2x}{3} - 4 = 4x + 4(4 - 4x) \) | \( x = \tfrac{30}{19} \) |
| \( \frac{2x}{3} + 2 = 2x + 2(2x + 2) \) | \( x = -\tfrac{3}{8} \) |
| \( 3x - 3(3 - x) = \frac{2x}{3} - 3 \) | \( x = \tfrac{9}{8} \) |
| \( \frac{2(2x - 1)}{3} + 2 = \frac{2x}{3} + 2(-4x - 4) \) | \( x = -\tfrac{14}{13} \) |
